formal/inference/heuristics/Store_Reuse_Subsumption.thy
@@ -4,127 +4,6 @@ begin
 
 declare One_nat_def [simp del]
 
-lemma medial_general_subset: "medial c (Guard (remove_guard_add_update t i r)) ra |\<subseteq>| medial c (Guard t) ra"
-  by (simp add: remove_guard_add_update_def medial_filter)
-
-lemma consistent_medial_generalisation: "consistent (medial c (Guard t)) \<Longrightarrow>
-                                         consistent (medial c (Guard (remove_guard_add_update t i r)))"
-  apply (simp add: consistent_def)
-  using medial_general_subset
-  by blast
-
-lemma get_medial_filter: "Contexts.get (medial c (filter f G)) x31 |\<subseteq>| Contexts.get (medial c G) x31"
-  apply (case_tac x31)
-     apply simp
-    apply (simp add: medial_filter)
-   apply (simp add: le_supI2 medial_filter sup.coboundedI1)
-  by (simp add: medial_filter)
-
-lemma fprod_get_medial_filter: "(a, b) |\<in>| Contexts.get (medial c (filter f G)) r |\<times>| Contexts.get (medial c (filter f G)) x32 \<Longrightarrow>
-                                (a, b) |\<in>| Contexts.get (medial c G) r |\<times>| Contexts.get (medial c G) x32"
-  using get_medial_filter
-  by (meson fin_mono fprod_subset)
-
-lemma apply_updates_filter: "Contexts.apply_updates (medial c (filter f G)) c U ra |\<subseteq>| Contexts.apply_updates (medial c G) c U ra"
-proof(induct U)
-  case Nil
-  then show ?case
-    by simp
-next
-  case (Cons a U)
-  then show ?case
-    apply (cases a)
-    apply (case_tac b)
-       apply simp
-      apply (simp add: medial_filter)
-     apply simp
-     apply clarify
-     apply simp
-    using fprod_get_medial_filter fimage_fprod apply metis
-     apply simp
-     apply clarify
-     apply simp
-    using fprod_get_medial_filter fimage_fprod by metis
-qed
-
-lemma guard2pairs_no_constraints_on_v: "\<not> gexp_constrains g1 (V v) \<Longrightarrow> list_all (\<lambda>(a, c). a \<noteq> V v) (guard2pairs c g1)"
-proof(induct g1)
-case (Bc x)
-  then show ?case
-    apply (case_tac x)
-    by auto
-next
-  case (Eq a1 a2)
-  then show ?case
-  proof(induct a1)
-    case (L x)
-    then show ?case
-      apply (induct a2)
-      by auto
-  next
-    case (V x)
-    then show ?case
-      apply (induct a2)
-      by auto
-  next
-    case (Plus a11 a12)
-    then show ?case
-      apply (induct a2)
-      by auto
-  next
-    case (Minus a11 a12)
-    then show ?case
-      apply (induct a2)
-      by auto
-  qed
-next
-  case (Gt a1 a2)
-  then show ?case
-  proof(induct a1)
-    case (L x)
-    then show ?case
-      by auto
-  next
-    case (V x)
-    then show ?case
-      apply (induct a2)
-      by auto
-  next
-    case (Plus a11 a12)
-    then show ?case
-      apply (induct a2)
-      by auto
-  next
-    case (Minus a11 a12)
-    then show ?case
-      apply (induct a2)
-      by auto
-  qed
-next
-  case (Null x)
-  then show ?case
-    by auto
-next
-case (Nor g11 g12)
-  then show ?case
-    apply simp
-    by (metis (mono_tags, lifting) Ball_set list.pred_map o_apply prod.sel(1) split_def)
-qed
-
-lemma pairs2context_no_constraints_on_v: "list_all (\<lambda>(a, c). a \<noteq> V v) l \<Longrightarrow> pairs2context l (V v) = {||}"
-proof-
-  assume premise: "list_all (\<lambda>(a, c). a \<noteq> V v) l"
-  have list_all_empty: "filter (\<lambda>(a, uu). a = V v) l = []"
-    using premise
-    by (simp add: Ball_set split_def)
-  show ?thesis
-    by (simp add: pairs2context_def list_all_empty)
-qed
-
-lemma pairs2context_no_constraints_on_v_2: "\<not> gexp_constrains g1 (V v) \<Longrightarrow> pairs2context (map (\<lambda>(x, y). (x, not |`| y)) (guard2pairs c g1)) (V v) = {||}"
-  using guard2pairs_no_constraints_on_v pairs2context_no_constraints_on_v
-  by (metis funion_absorb gexp_constrains.simps(5) guard2pairs.simps(30) map_append pairs2context_append)
-
 lemma generalisation_of_preserves: "is_generalisation_of t' t i r \<Longrightarrow>
     Label t = Label t' \<and>
     Arity t = Arity t' \<and>
@@ -132,327 +11,58 @@ lemma generalisation_of_preserves: "is_generalisation_of t' t i r \<Longrightarr
   apply (simp add: is_generalisation_of_def)
   using remove_guard_add_update_preserves by auto
 
-lemma generalisation_medial_subset: "is_generalisation_of t' t i r \<Longrightarrow> medial c (Guard t') a |\<subseteq>| medial c (Guard t) a"
-  apply (simp add: is_generalisation_of_def)
-  using medial_general_subset by blast
+lemma is_generalisation_of_guard_subset: "is_generalisation_of t' t i r \<Longrightarrow> set (Guard t') \<subseteq> set (Guard t)"
+  apply (simp add: is_generalisation_of_def remove_guard_add_update_def)
+  by auto
 
-lemma generalisation_medial_equiv: "is_generalisation_of t' t i r \<Longrightarrow> medial c (Guard t @ Guard t') = medial c (Guard t)"
-  apply (rule ext)
-  apply (simp add: is_generalisation_of_def medial_append)
-  using medial_general_subset by blast
+lemma is_generalisation_of_medial: "is_generalisation_of t' t i r \<Longrightarrow> can_take t ip rg \<longrightarrow> can_take t' ip rg"
+  using is_generalisation_of_guard_subset medial_subset by blast
 
-lemma apply_updates_same: "\<forall>i. c (V (I i)) = {|Bc True|} \<Longrightarrow>
-       \<forall>i. \<forall>u\<in>set U. fst u \<noteq> v \<and> fst u \<noteq> I i \<Longrightarrow>
-       consistent (medial c (Guard t)) \<Longrightarrow>
-       remove_obsolete_constraints (Contexts.apply_updates (medial c (Guard t)) c U) (fst |`| fset_of_list U) (V v) = c (V v)"
-proof(induct U)
-  case Nil
-  then show ?case
-    apply (simp add: remove_obsolete_constraints_def)
-    by auto
-next
-  case (Cons u us)
-  then show ?case
-    apply (cases u)
-    apply (simp add: remove_obsolete_constraints_def)
-    apply (case_tac v)
-     apply simp
-    apply simp
-    apply clarify
-    apply standard
-     apply (metis (no_types, lifting) empty_variable_constraints)
-    apply (case_tac b)
-       apply simp
-       apply (smt fBexE)
-      apply simp
-      apply (smt fBexE)
-     apply simp
-     apply (smt fBexE)
-    apply simp
-    by (smt fBexE)
-qed
+lemma is_generalisation_of_preserves_reg: 
+  "is_generalisation_of t' t i r \<Longrightarrow>
+   apply_updates (Updates t) c (d2r c) r = c (R r)"
+  by (simp add: is_generalisation_of_def r_not_updated_stays_the_same)
 
-lemma posterior_same: "\<forall>i. c (V (I i)) = {|Bc True|} \<Longrightarrow>
-       \<forall>i. \<forall>u\<in>set (Updates t). fst u \<noteq> v \<and> fst u \<noteq> I i \<Longrightarrow>
-       consistent (medial c (Guard t)) \<Longrightarrow>
-       posterior c t (V v) = c (V v)"
-  by (simp add: posterior_def posterior_separate_def apply_updates_same)
-
-lemma is_generalisation_of_consistent_medial: "is_generalisation_of t' t i r \<Longrightarrow>
-    consistent (medial c (Guard t)) \<Longrightarrow> 
-    consistent (medial c (Guard t'))"
-  by (simp add: is_generalisation_of_def consistent_medial_generalisation)
-
-lemma is_generalisation_of_posterior_subset: "is_generalisation_of t' t i r \<Longrightarrow> a \<noteq> V (R r) \<Longrightarrow>
-       consistent (medial c (Guard t)) \<Longrightarrow>
-       posterior c t' a |\<subseteq>| posterior c t a"
-  apply (simp add: posterior_def posterior_separate_def)
-  apply (simp add: Let_def generalisation_medial_equiv)
-   apply (simp add: is_generalisation_of_consistent_medial)
-   apply (simp add: is_generalisation_of_def remove_guard_add_update_def)
-   apply (simp add: remove_obsolete_constraints_def)
-   apply standard
-    apply auto[1]
-  by (simp add: apply_updates_filter)
-
-lemma posterior_Rr_undef: "\<forall>i. c (V (I i)) = {|Bc True|} \<Longrightarrow>
-       c (V (R r)) = {|Undef|} \<Longrightarrow>
-       \<forall>i. \<forall>u\<in>set (Updates t). fst u \<noteq> R r \<and> fst u \<noteq> I i \<Longrightarrow>
-       consistent (medial c (Guard t)) \<Longrightarrow>
-       posterior c t (V (R r)) = {|Undef|}"
-  by (simp add: posterior_same)
-
-lemma aux2: "is_generalisation_of t' t i r \<Longrightarrow>
-       c (V (R r)) = {|Undef|} \<Longrightarrow>
-       \<forall>i. c (V (I i)) = {|Bc True|} \<Longrightarrow>
-       \<forall>i. \<forall>u\<in>set (Updates t). fst u \<noteq> R r \<and> fst u \<noteq> I i \<Longrightarrow>
-       fBall (Contexts.apply_updates (medial c (Guard t)) c (Updates t') ra) (\<lambda>c. cval c ra ia = true) \<Longrightarrow>
-       Contexts.apply_updates (medial c (Guard t)) c (Updates t) ra \<noteq> {|Undef|} \<Longrightarrow>
-       x |\<in>| Contexts.apply_updates (medial c (Guard t)) c (Updates t) ra \<Longrightarrow>
-       consistent (medial c (Guard t)) \<Longrightarrow> ra \<noteq> V (R r) \<Longrightarrow> \<forall>n. \<not> aexp_constrains ra (V (I n)) \<Longrightarrow> cval x ra ia = true"
-proof(induct "Updates t")
-case Nil
-  then show ?case
-    apply (simp add: is_generalisation_of_def remove_guard_add_update_def)
-    by auto
-next
-  case (Cons u us)
-  then show ?case
-    apply (simp add: is_generalisation_of_def remove_guard_add_update_def)
-    by auto
-qed
-
-lemma generalised_updates:  "is_generalisation_of t' t i r \<Longrightarrow> Updates t' = (R r, (V (I i)))#(Updates t)"
+lemma is_generalisation_of_preserves_reg_2: "is_generalisation_of t' t i r \<Longrightarrow> ra \<noteq> r \<Longrightarrow> apply_updates (Updates t') (join_ir ia c) (d2r (join_ir ia c)) ra = apply_updates (Updates t) (join_ir ia c) (d2r (join_ir ia c)) ra"
   by (simp add: is_generalisation_of_def remove_guard_add_update_def)
 
-lemma aux3: "\<not> gexp_constrains a (V v) \<Longrightarrow> pairs2context (guard2pairs c a) (V v) |\<subseteq>| c (V v)"
-proof(induct a)
-case (Bc x)
-  then show ?case
-    apply (case_tac x)
-     apply (simp add: pairs2context_def)
-    by(simp add: pairs2context_def)
-next
-  case (Eq a1 a2)
-  then show ?case
-  proof(induct a1)
-    case (L x)
-    then show ?case
-      apply (induct a2)
-      using pairs2context_def
-      by auto
-  next
-    case (V x)
-    then show ?case
-      apply (induct a2)
-      using pairs2context_def
-      by auto
-  next
-    case (Plus a11 a12)
-    then show ?case
-      apply (induct a2)
-      using pairs2context_def
-      by auto
-  next
-    case (Minus a11 a12)
-    then show ?case
-      apply (induct a2)
-      using pairs2context_def
-      by auto
-  qed
-next
-  case (Gt a1 a2)
-  then show ?case
-  proof(induct a1)
-    case (L x)
-    then show ?case
-      apply (induct a2)
-      using pairs2context_def
-      by auto
-  next
-    case (V x)
-    then show ?case
-      apply (induct a2)
-      using pairs2context_def
-      by auto
-  next
-    case (Plus a11 a12)
-    then show ?case 
-      apply (induct a2)
-      using pairs2context_def
-      by auto
-  next
-    case (Minus a11 a12)
-    then show ?case 
-      apply (induct a2)
-      using pairs2context_def
-      by auto
-  qed
-next
-  case (Nor a1 a2)
-  then show ?case
-    apply (simp add: pairs2context_append)
-    apply standard
-     apply (simp add: pairs2context_no_constraints_on_v_2)
-    by (simp add: pairs2context_no_constraints_on_v_2)
-next
-  case (Null x)
-  then show ?case
-    apply (simp add: pairs2context_def)
-    by auto
-qed
-
-lemma medial_filter_constraints: "medial c (filter (\<lambda>g. \<not> gexp_constrains g (V (I i))) G) (V (I i)) = c (V (I i))"
-proof(induct G)
-  case Nil
-  then show ?case
-    by (simp add: medial_def pairs2context_def List.maps_def)
-next
-  case (Cons a G)
-  then show ?case
-    apply (simp add: medial_def List.maps_simps pairs2context_append)
-    apply standard
-    apply standard
-     prefer 2
-     apply blast
-    apply simp
-    apply standard
-    defer
-     apply auto[1]
-    by (simp add: aux3)
-qed
-
-lemma generealisation_medial: "is_generalisation_of t' t i r \<Longrightarrow>
-       medial c (Guard t') (V (I i)) = c (V (I i))"
-  apply (simp add: is_generalisation_of_def remove_guard_add_update_def)
-  by (simp add: medial_filter_constraints)
-
-lemma generalisation_posterior_consistent: "is_generalisation_of t' t i r \<Longrightarrow>
-       c (V (R r)) = {|Undef|} \<Longrightarrow>
-       \<forall>i. c (V (I i)) = {|Bc True|} \<Longrightarrow>
-       \<forall>i. \<forall>u\<in>set (Updates t). fst u \<noteq> R r \<and> fst u \<noteq> I i \<Longrightarrow>
-       consistent (medial c (Guard t)) \<Longrightarrow>
-       fBall (posterior c t a) (\<lambda>c. cval c a s = true) \<Longrightarrow>
-       fBall (posterior c t' a) (\<lambda>c. cval c a s = true)"
-  apply (case_tac "a \<noteq> V (R r)")
-  using is_generalisation_of_posterior_subset apply blast
-  apply (simp add: posterior_def posterior_separate_def Let_def is_generalisation_of_consistent_medial)
-  apply (simp add: generalised_updates remove_obsolete_constraints_def)
-  apply (case_tac "fBex (fset_of_list (Updates t)) (\<lambda>x. fst x = R r \<and> R r \<noteq> fst x)")
-   apply auto[1]
-  apply simp
-  apply standard
-   apply auto[1]
-  apply clarify
-  by (simp add: generealisation_medial cval_true)
+lemma is_generalisation_of_apply_guards: "is_generalisation_of t' t i r \<Longrightarrow>
+       apply_guards (Guard t) (join_ir ia c) \<Longrightarrow>
+       apply_guards (Guard t') (join_ir ia c)"
+  using is_generalisation_of_guard_subset apply_guards_subset by blast
 
 (*
   This shows that if we drop the guard and add an update, and the updated register is undefined
   in the context, c, then the generalised transition subsumes the specific one
 *)
-lemma is_generalisation_of_subsumes_original: "is_generalisation_of t' t i r \<Longrightarrow>
-                                               c (V (R r)) = {|Undef|} \<Longrightarrow>
-                                               \<forall>i. c (V (I i)) = {|Bc True|} \<Longrightarrow>
-                                               \<forall>i. \<forall>u \<in> set (Updates t). fst u \<noteq> (R r) \<and> fst u \<noteq> (I i) \<Longrightarrow>
-                                               t' \<^sub>c\<sqsupseteq> t"
-    apply (rule subsumption)
-       apply (simp add: generalisation_of_preserves)
-  using generalisation_medial_subset apply blast
-     apply (simp add: generalisation_of_preserves)
-    apply (simp add: generalisation_of_preserves)
-   apply clarify
-   apply (case_tac "consistent (medial c (Guard t))")
-    prefer 2
-    apply (simp add: posterior_def posterior_separate_def Let_def generalisation_medial_equiv)
-
-   apply (case_tac "ra = V (R r)")
-    apply clarify
-    apply (simp add: posterior_Rr_undef)
-   apply (simp add: posterior_separate_def posterior_def Let_def generalisation_medial_equiv remove_obsolete_constraints_def)
-   apply (case_tac "(\<exists>n. aexp_constrains ra (V (I n)))")
-    apply auto[1]
-   apply (case_tac "fBex (fset_of_list (Updates t')) (\<lambda>x. V (fst x) = ra \<and> ra \<noteq> V (fst x))")
-    apply auto[1]
-   apply (case_tac "fBex (fset_of_list (Updates t)) (\<lambda>x. V (fst x) = ra \<and> ra \<noteq> V (fst x))")
-    apply auto[1]
-   apply simp
-   apply (simp add: aux2)
-
-  apply (simp only: consistent_def)
+lemma is_generalisation_of_subsumes_original:
+  "is_generalisation_of t' t i r \<Longrightarrow>
+   c r = None \<Longrightarrow>
+   subsumes t' c t"
+  apply (rule subsumption)
+      apply (simp add: is_generalisation_of_def remove_guard_add_update_def)
+     apply (simp add: is_generalisation_of_medial)
+    apply (simp add: is_generalisation_of_def remove_guard_add_update_def)
+   apply (simp add: posterior_def)
   apply clarify
-  apply (rule_tac x=s in exI)
-
-  apply (case_tac "consistent (medial c (Guard t))")
-   apply (simp add: generalisation_posterior_consistent)
-
-  apply (simp add: posterior_def posterior_separate_def Let_def)
+   apply (case_tac "ra = r")
+    apply (simp add: is_generalisation_of_preserves_reg join_ir_def)
+   apply (simp add: is_generalisation_of_preserves_reg_2)
   apply clarify
-  by (simp add: cval_false)
-
-lemma restrict_value_of_register: "c (V (R r)) = {|cexp.Eq v|} \<Longrightarrow>
-       consistent (\<lambda>x. datastate2context ra x |\<union>| c x) \<Longrightarrow>
-       ra (R r) = Some v"
-proof-
-  assume premise1: "c (V (R r)) = {|cexp.Eq v|}"
-  assume premise2: "consistent (\<lambda>x. datastate2context ra x |\<union>| c x)"
-  have contra: "\<And>c r v ra. c (V (R r)) = {|cexp.Eq v|} \<Longrightarrow>
-       ra (R r) \<noteq> Some v \<Longrightarrow>
-       \<not> consistent (\<lambda>x. datastate2context ra x |\<union>| c x)"
-  apply (simp add: datastate2context_def consistent_def)
-  apply clarify
-  apply (rule_tac x="V (R r)" in exI)
-  apply simp
-  apply (simp add: cval_def gval.simps ValueEq_def)
-  apply (case_tac "ra (R r)")
-   apply (simp add: gval.simps ValueEq_def)
-    by (simp add: gval.simps ValueEq_def)
-  show ?thesis
-    using contra premise1 premise2
-    by auto
-qed
-
-lemma length_apply_generalised_outputs: "length (apply_outputs (Outputs t)                         (case_vname (\<lambda>n. input2state i 1 (I n)) (\<lambda>n. ra (R n)))) =
-                                         length (apply_outputs (Outputs (generalise_output t p r)) (case_vname (\<lambda>n. input2state i 1 (I n)) (\<lambda>n. ra (R n))))"
-  by (simp add: apply_outputs_alt generalise_output_preserves_output_length)
-
-lemma apply_outputs_equiv: "i < length (Outputs t) \<Longrightarrow>
-       i \<noteq> r \<Longrightarrow>
-       (apply_outputs (Outputs t) s) ! i = (apply_outputs (Outputs (generalise_output t p r)) s) ! i"
-  apply (simp add: generalise_output_def)
-  by (simp add: apply_outputs_alt)
+  apply (simp add: posterior_def)
+  apply (case_tac "apply_guards (Guard t) (join_ir ia c)")
+   apply (simp add: is_generalisation_of_apply_guards)
+   apply (metis is_generalisation_of_preserves_reg is_generalisation_of_preserves_reg_2 join_ir_def option.simps(3) vname.simps(6))
+  by simp
 
 (* 
   This shows that if we can guarantee that the value of a particular register is the literal output
   then the generalised output subsumes the specific output
 *)
-
 lemma generalise_output_subsumes_original: "nth (Outputs t) r = L v \<Longrightarrow>
-                                            c (V (R p)) = {|Eq v|} \<Longrightarrow>
-                                            generalise_output t p r \<^sub>c\<sqsupseteq> t"
-  apply (simp add: subsumes_def generalise_output_preserves)
-  apply standard
-   apply (simp add: satisfies_context_def)
-   apply clarify
-   apply (simp add: list_eq_iff_nth_eq length_apply_generalised_outputs )
-   apply clarify
-   apply (simp only: apply_outputs_preserves_length)
-   apply (case_tac "ia = r")
-    prefer 2
-    apply (simp add: apply_outputs_equiv)
-   apply (simp add: apply_outputs_alt generalise_output_def)
-   apply (simp add: restrict_value_of_register)
-  apply standard
-   apply (simp add: list_eq_iff_nth_eq length_apply_generalised_outputs apply_outputs_alt generalise_output_def)
-   apply (rule_tac x=i in exI)
-   apply (rule_tac x="<R p := v>" in exI)
-   apply (rule allI)
-   apply (case_tac "ia = r")
-    apply simp
-   apply simp
-  apply standard
-  apply (rule allI)+
-   apply (simp add: posterior_separate_append_self posterior_def generalise_output_preserves)
-  by (simp add: posterior_def posterior_separate_def  generalise_output_preserves)
+                                            c p = Some v \<Longrightarrow>
+                                            subsumes (generalise_output t p r) (r2d c) t"
+  oops
 
 primrec stored_reused_aux_per_reg :: "transition \<Rightarrow> transition \<Rightarrow> nat \<Rightarrow> nat \<Rightarrow> (nat \<times> nat) option" where
   "stored_reused_aux_per_reg t' t 0 p = (if is_generalised_output_of t' t 0 p then Some (0, p) else None)" |
